Util/Vector/VecOrd.v
@@ -7,7 +7,7 @@ See the COPYRIGHTS and LICENSE files.
 symmetric product on vectors
 ************************************************************************)
 
-(* $Id: VecOrd.v,v 1.2 2006-12-01 09:37:48 blanqui Exp $ *)
+(* $Id: VecOrd.v,v 1.3 2006-12-04 12:53:52 blanqui Exp $ *)
 
 Set Implicit Arguments.
 
@@ -16,11 +16,11 @@ Require Export VecUtil.
 
 Section S.
 
-Variables (A : Set) (ltA : A->A->Prop).
+Variables (A : Set) (gtA : A->A->Prop).
 
 Notation vec := (vector A).
 
-Infix "<A" := ltA (at level 70).
+Infix ">A" := gtA (at level 70).
 
 (* product ordering *)
 
@@ -28,18 +28,18 @@ Require Export Relations.
 
 Implicit Arguments symprod [A B].
 
-Fixpoint Vlt_prod n : vec n -> vec n -> Prop :=
+Fixpoint Vgt_prod n : vec n -> vec n -> Prop :=
   match n as n return vec n -> vec n -> Prop with
     | O => fun _ _ => False
-    | S n => fun v1 v2 => symprod ltA (@Vlt_prod n) (Vsplit v1) (Vsplit v2)
+    | S n => fun v1 v2 => symprod gtA (@Vgt_prod n) (Vsplit v1) (Vsplit v2)
   end.
 
-Infix "<prod" := Vlt_prod (at level 70).
+Infix ">prod" := Vgt_prod (at level 70).
 
-Lemma Vlt_prod_lt : forall n (v1 v2 : vec n), v1 <prod v2 -> exists i,
+Lemma Vgt_prod_gt : forall n (v1 v2 : vec n), v1 >prod v2 -> exists i,
   exists vi : vec i, exists x, exists j, exists vj : vec j, exists h, exists y,
   v1 = Vcast (Vapp vi (Vcons x vj)) h /\ v2 = Vcast (Vapp vi (Vcons y vj)) h
-  /\ x <A y.
+  /\ x >A y.
 
 Proof.
 induction v1; simpl. intros. contradiction. intro. VSntac v2.
@@ -55,9 +55,9 @@ simpl. intuition. apply Vcons_eq_tail. apply Vcast_eq.
 apply Vcons_eq_tail. apply Vcast_eq.
 Qed.
 
-Lemma Vlt_prod_cons : forall x1 x2 n (v1 v2 : vec n),
-  (x1 <A x2 /\ v1 = v2) \/ (x1 = x2 /\ v1 <prod v2)
-  -> Vcons x1 v1 <prod Vcons x2 v2.
+Lemma Vgt_prod_cons : forall x1 x2 n (v1 v2 : vec n),
+  (x1 >A x2 /\ v1 = v2) \/ (x1 = x2 /\ v1 >prod v2)
+  -> Vcons x1 v1 >prod Vcons x2 v2.
 
 Proof.
 intros. simpl. unfold Vsplit. simpl. destruct H; destruct H.
@@ -65,25 +65,25 @@ subst v2. apply left_sym. assumption.
 subst x2. apply right_sym. assumption.
 Qed.
 
-Lemma Vlt_prod_inv : forall x1 x2 n (v1 v2 : vec n),
-  Vcons x1 v1 <prod Vcons x2 v2 ->
-  (x1 <A x2 /\ v1 = v2) \/ (x1 = x2 /\ v1 <prod v2).
+Lemma Vgt_prod_inv : forall x1 x2 n (v1 v2 : vec n),
+  Vcons x1 v1 >prod Vcons x2 v2 ->
+  (x1 >A x2 /\ v1 = v2) \/ (x1 = x2 /\ v1 >prod v2).
 
 Proof.
 intros. simpl in H. unfold Vsplit in H. simpl in H. inversion H.
 left. auto. right. auto.
 Qed.
 
-Lemma Vlt_prod_app : forall n (v : vec n) m (v1 v2 : vec m),
-  v1 <prod v2 -> Vapp v v1 <prod Vapp v v2.
+Lemma Vgt_prod_app : forall n (v : vec n) m (v1 v2 : vec m),
+  v1 >prod v2 -> Vapp v v1 >prod Vapp v v2.
 
 Proof.
 induction v; intros. assumption.
 simpl. unfold Vsplit. simpl. apply right_sym. apply IHv. assumption.
 Qed.
 
-Lemma Vlt_prod_cast : forall m n (h : m=n) (v1 v2 : vec m),
-  v1 <prod v2 -> Vcast v1 h <prod Vcast v2 h.
+Lemma Vgt_prod_cast : forall m n (h : m=n) (v1 v2 : vec m),
+  v1 >prod v2 -> Vcast v1 h >prod Vcast v2 h.
 
 Proof.
 induction v1; intros; destruct n; intros.
@@ -93,8 +93,8 @@ assert (h = refl_equal (S n)). apply UIP. subst h.
 rewrite (Vcast_refl_eq (Vcons a v1)). rewrite (Vcast_refl_eq v2). assumption.
 Qed.
 
-Lemma Vlt_prod_cast_inv : forall m n (h : m=n) (v1 v2 : vec m),
-  Vcast v1 h <prod Vcast v2 h -> v1 <prod v2.
+Lemma Vgt_prod_cast_inv : forall m n (h : m=n) (v1 v2 : vec m),
+  Vcast v1 h >prod Vcast v2 h -> v1 >prod v2.
 
 Proof.
 induction m; destruct n; intros.
@@ -103,67 +103,67 @@ discriminate. discriminate.
 assert (v1 = Vcons (Vhead v1) (Vtail v1)). apply VSn_eq. rewrite H0.
 assert (v2 = Vcons (Vhead v2) (Vtail v2)). apply VSn_eq. rewrite H1.
 rewrite H0 in H. rewrite H1 in H. simpl in H. unfold Vsplit in H. simpl in H.
-apply Vlt_prod_cons. inversion H. left. split. assumption.
+apply Vgt_prod_cons. inversion H. left. split. assumption.
 eapply Vcast_eq_intro with (m := n). apply H6.
 right. split. reflexivity. eapply IHm with (n := n). apply H3.
 Qed.
 
-Require Export Wellfounded.
+Require Export SN.
 
-Lemma Vforall_Acc_lt_prod : forall n (v : vec n),
-  Vforall (Acc ltA) v -> Acc (@Vlt_prod n) v.
+Lemma Vforall_SN_gt_prod : forall n (v : vec n),
+  Vforall (SN gtA) v -> SN (@Vgt_prod n) v.
 
 Proof.
-induction v; intros; apply Acc_intro; intros. contradiction.
-simpl. eapply Acc_inverse_image with (R := symprod ltA (@Vlt_prod n)).
+induction v; intros; apply SN_intro; intros. contradiction.
+simpl. eapply SN_inverse with (R := symprod gtA (@Vgt_prod n)).
 VSntac y. unfold Vsplit. simpl. simpl in H. destruct H.
 rewrite H1 in H0. inversion H0.
-apply Acc_symprod. eapply Acc_inv. apply H. assumption.
-rewrite H7. apply IHv. assumption.
-apply Acc_symprod. rewrite H6. assumption.
-eapply Acc_inv. apply IHv. apply H2. assumption.
+apply SN_symprod. eapply SN_inv. apply H. assumption.
+rewrite <- H7. apply IHv. assumption.
+apply SN_symprod. rewrite <- H6. assumption.
+eapply SN_inv. apply IHv. apply H2. assumption.
 Qed.
 
-Lemma Acc_lt_prod_Sn_head : forall n (v : vec (S n)),
-  Acc (@Vlt_prod (S n)) v -> Acc ltA (Vhead v).
+Lemma SN_gt_prod_Sn_head : forall n (v : vec (S n)),
+  SN (@Vgt_prod (S n)) v -> SN gtA (Vhead v).
 
 Proof.
-induction 1. VSntac x. apply Acc_intro. intros.
+induction 1. VSntac x. apply SN_intro. intros.
 deduce (H0 (Vcons y (Vtail x))). apply H3. rewrite H1. simpl.
 unfold Vsplit. simpl. apply left_sym. assumption.
 Qed.
 
-Lemma Acc_lt_prod_head : forall a n (v : vec n),
-  Acc (@Vlt_prod (S n)) (Vcons a v) -> Acc ltA a.
+Lemma SN_gt_prod_head : forall a n (v : vec n),
+  SN (@Vgt_prod (S n)) (Vcons a v) -> SN gtA a.
 
 Proof.
-intros. deduce (Acc_lt_prod_Sn_head H). assumption.
+intros. deduce (SN_gt_prod_Sn_head H). assumption.
 Qed.
 
-Lemma Acc_lt_prod_Sn_tail : forall n (v : vec (S n)),
-  Acc (@Vlt_prod (S n)) v -> Acc (@Vlt_prod n) (Vtail v).
+Lemma SN_gt_prod_Sn_tail : forall n (v : vec (S n)),
+  SN (@Vgt_prod (S n)) v -> SN (@Vgt_prod n) (Vtail v).
 
 Proof.
-induction 1. VSntac x. apply Acc_intro. intros.
+induction 1. VSntac x. apply SN_intro. intros.
 deduce (H0 (Vcons (Vhead x) y)). rewrite H1 in H3. apply H3.
 simpl. unfold Vsplit. simpl. apply right_sym. assumption.
 Qed.
 
-Lemma Acc_lt_prod_tail : forall a n (v : vec n),
-  Acc (@Vlt_prod (S n)) (Vcons a v) -> Acc (@Vlt_prod n) v.
+Lemma SN_gt_prod_tail : forall a n (v : vec n),
+  SN (@Vgt_prod (S n)) (Vcons a v) -> SN (@Vgt_prod n) v.
 
 Proof.
-intros. deduce (Acc_lt_prod_Sn_tail H). assumption.
+intros. deduce (SN_gt_prod_Sn_tail H). assumption.
 Qed.
 
-Lemma Acc_lt_prod_forall : forall n (v : vec n),
-  Acc (@Vlt_prod n) v -> Vforall (Acc ltA) v.
+Lemma SN_gt_prod_forall : forall n (v : vec n),
+  SN (@Vgt_prod n) v -> Vforall (SN gtA) v.
 
 Proof.
 induction v; intros; simpl. exact I. split.
-apply (Acc_lt_prod_head H). apply IHv. apply (Acc_lt_prod_tail H).
+apply (SN_gt_prod_head H). apply IHv. apply (SN_gt_prod_tail H).
 Qed.
 
 End S.
 
-Implicit Arguments Vlt_prod_lt [A ltA n v1 v2].
+Implicit Arguments Vgt_prod_gt [A gtA n v1 v2].
