Term/WithArity/ASN.v
@@ -8,7 +8,7 @@ See the COPYRIGHTS and LICENSE files.
 general results on the strong normalization of rewrite relations
 ************************************************************************)
 
-(* $Id: ASN.v,v 1.2 2006-12-01 09:37:48 blanqui Exp $ *)
+(* $Id: ASN.v,v 1.3 2006-12-04 12:53:52 blanqui Exp $ *)
 
 Set Implicit Arguments.
 
@@ -32,31 +32,33 @@ Variable R : rules.
 
 Notation Red := (@red Sig R).
 
-Notation SN := (Acc (transp Red)).
+Require Export SN.
+
+Notation SNR := (SN Red).
 
 (***********************************************************************)
 (* every subterm of an sn term is sn *)
 
-Lemma subterm_sn : forall t, SN t -> forall u, subterm_eq u t -> SN u.
+Lemma subterm_sn : forall t, SNR t -> forall u, subterm_eq u t -> SNR u.
 
 Proof.
-intros t H. elim H. clear t H. intros t H IH u H0. apply Acc_intro.
+intros t H. elim H. clear t H. intros t H IH u H0. apply SN_intro.
 intros u' H1. deduce (red_subterm H1 H0). destruct H2 as [t']. destruct H2.
-eapply IH. unfold transp. apply H2. assumption.
+eapply IH. apply H2. assumption.
 Qed.
 
-Lemma sub_sn : forall l x s, In x (varlist l) -> SN (app s l) -> SN (s x).
+Lemma sub_sn : forall l x s, In x (varlist l) -> SNR (app s l) -> SNR (s x).
 
 Proof.
-intros. change (SN (app s (Var x))). eapply subterm_sn. apply H0.
+intros. change (SNR (app s (Var x))). eapply subterm_sn. apply H0.
 apply subterm_app. apply in_varlist_subterm. assumption.
 Qed.
 
 Lemma sub_fun_sn : forall f ts x s,
-  In x (varlist (Fun f ts)) -> Vforall SN (Vmap (app s) ts) -> SN (s x).
+  In x (varlist (Fun f ts)) -> Vforall SNR (Vmap (app s) ts) -> SNR (s x).
 
 Proof.
-intros. change (SN (app s (Var x))). rewrite varlist_fun in H.
+intros. change (SNR (app s (Var x))). rewrite varlist_fun in H.
 deduce (in_varlists H). destruct H1 as [t]. destruct H1.
 deduce (in_varlist_subterm H2). apply subterm_sn with (t := app s t).
 eapply Vforall_in with (n := arity f). apply H0. apply Vin_map_elim. assumption.
@@ -80,10 +82,10 @@ Qed.
 (***********************************************************************)
 (* variables are sn *)
 
-Lemma sn_var : forall v, SN (Var v).
+Lemma sn_var : forall v, SNR (Var v).
 
 Proof.
-intro. apply Acc_intro. intros t H. redtac. absurd (@notvar Sig (Var v)).
+intro. apply SN_intro. intros t H. redtac. absurd (@notvar Sig (Var v)).
 apply notvar_var. rewrite H0. apply notvar_fillapp. eapply hyp1. apply H.
 Qed.
 
@@ -93,13 +95,13 @@ Qed.
 Require Export ACalls.
 
 Lemma sn_args_sn_fun : forall f, defined f R = false ->
-  forall ts, Vforall SN ts -> SN (Fun f ts).
+  forall ts, Vforall SNR ts -> SNR (Fun f ts).
 
 Proof.
-intros. set (lt := (@Vlt_prod term (transp Red) (arity f))).
-assert (Acc lt ts). unfold lt. apply Vforall_Acc_lt_prod. assumption.
+intros. set (gt := (@Vgt_prod term Red (arity f))).
+assert (SN gt ts). unfold gt. apply Vforall_SN_gt_prod. assumption.
 elim H1. intros.
-apply Acc_intro. change (forall y, Red (Fun f x) y -> SN y). intros.
+apply SN_intro. change (forall y, Red (Fun f x) y -> SNR y). intros.
 redtac. subst y. destruct c; simpl in H5; simpl.
 (* C = Hole *)
 case (fun_eq_app H5); intro H6; destruct H6.
@@ -109,16 +111,15 @@ eapply lhs_fun_defined. apply H6. apply H4.
 (* lhs is Var *)
 absurd (l = Var x0). eapply lhs_notvar. apply H4. assumption.
 (* C <> Hole *)
-Funeqtac. subst x. apply H3. unfold lt. eapply Vlt_prod_cast. apply Vlt_prod_app.
-apply Vlt_prod_cons. left. split. 2: reflexivity.
-unfold transp. apply red_rule. assumption.
+Funeqtac. subst x. apply H3. unfold gt. eapply Vgt_prod_cast. apply Vgt_prod_app.
+apply Vgt_prod_cons. left. split. 2: reflexivity. apply red_rule. assumption.
 Qed.
 
 (***********************************************************************)
 (* application of an sn substitution to a term without defined symbols *)
 
 Lemma no_call_app_sn : forall t, calls R t = nil -> forall s,
-  (forall x, In x (varlist t) -> SN (s x)) -> SN (app s t).
+  (forall x, In x (varlist t) -> SNR (s x)) -> SNR (app s t).
 
 Proof.
 intro. pattern t. apply term_ind_forall; clear t; intros.
@@ -140,14 +141,14 @@ then [app s (Fun g vs)] is sn whenever [Gun g vs] is a call in [r] *)
 
 Require Export ACap.
 
-Lemma calls_sn_args : forall r s, (forall x, In x (varlist r) -> SN (s x))
+Lemma calls_sn_args : forall r s, (forall x, In x (varlist r) -> SNR (s x))
   -> (forall g vs, In (Fun g vs) (calls R r)
-                   -> Vforall SN (Vmap (app s) vs) -> SN (app s (Fun g vs)))
-  -> forall g vs, In (Fun g vs) (calls R r) -> Vforall SN (Vmap (app s) vs).
+                   -> Vforall SNR (Vmap (app s) vs) -> SNR (app s (Fun g vs)))
+  -> forall g vs, In (Fun g vs) (calls R r) -> Vforall SNR (Vmap (app s) vs).
 
 Proof.
 intros r s H H0. cut (forall a g vs, a = Fun g vs
-  -> In a (calls R r) -> Vforall SN (Vmap (app s) vs)).
+  -> In a (calls R r) -> Vforall SNR (Vmap (app s) vs)).
 intros. apply H1 with (a := Fun g vs). refl. assumption.
 intro a. pattern a. apply subterm_ind. clear a. intros. subst t.
 apply Vforall_elim. intros w H2.
@@ -179,10 +180,10 @@ eapply subterm_trans_eq1. eapply in_calls_subterm. apply H11.
 apply subterm_fun. assumption. refl. assumption.
 Qed.
 
-Lemma calls_sn : forall r s, (forall x, In x (varlist r) -> SN (s x))
+Lemma calls_sn : forall r s, (forall x, In x (varlist r) -> SNR (s x))
   -> (forall g vs, In (Fun g vs) (calls R r)
-                   -> Vforall SN (Vmap (app s) vs) -> SN (app s (Fun g vs)))
-  -> forall a, In a (calls R r) -> SN (app s a).
+                   -> Vforall SNR (Vmap (app s) vs) -> SNR (app s (Fun g vs)))
+  -> forall a, In a (calls R r) -> SNR (app s a).
 
 Proof.
 intros. deduce (in_calls H1). destruct H2 as [g]. destruct H2 as [vs].
